BitVectors.v
@@ -1,0 +1,355 @@
+Require Import NArith.
+
+Require Import Lia.
+
+Require Import UROP.Types.
+Require Import UROP.ExtraArith.
+Require Import UROP.Tactics.
+
+Local Open Scope UROP_scope.
+
+
+(* List Helper Lemmas {{{ *)
+Local Open Scope N_scope.
+Lemma list_fact {A} : forall n m (l : list A) d,
+  lt n m
+  -> ge (List.length l) m
+  -> List.nth n (List.firstn m l) d = List.nth n l d.
+Proof.
+  intros.
+  replace (List.nth n l d) with (List.nth n (List.firstn m l ++l List.skipn m l) d).
+  Search (List.nth).
+  rewrite List.app_nth1; eauto.
+  rewrite List.firstn_length; lia.
+  rewrite List.firstn_skipn; eauto.
+Qed.
+
+Lemma rev_rev {A} : forall (l : list A),
+  List.NoDup (List.rev l) -> List.NoDup l.
+Proof.
+  intros.
+  apply List.NoDup_rev in H.
+  rewrite List.rev_involutive in H.
+  assumption.
+Qed.
+
+Open Scope list_scope.
+Lemma zip_app {A} {B} : forall (a1 : list A) (b1 : list B) a2 b2,
+  List.length a1 = List.length b1
+  -> zip (a1 ++ a2) (b1 ++ b2) = zip a1 b1 ++ zip a2 b2.
+Proof.
+  induction a1; induction b1; eauto.
+  inversion 1.
+  inversion 1.
+  intros; simpl.
+  f_equal.
+  eauto.
+Qed.
+
+Lemma zip_length {A} {B} : forall (a : list A) (b : list B),
+  List.length (zip a b) = Nat.min (List.length a) (List.length b).
+Proof.
+  induction a; induction b; simpl; eauto.
+Qed.
+Close Scope list_scope.
+
+Lemma list_firstn_skipn_succ : forall A (l : list A) i d,
+  lt i (List.length l) ->
+  List.skipn i (List.firstn (i+1) l) = [List.nth i l d].
+Proof.
+  induction l.
+  inversion 1.
+
+  lists.
+  intros.
+  destruct i.
+  lists.
+  replace ((S i + 1)%nat) with (S (i + 1)) by lia.
+  lists.
+  apply IHl.
+  lia.
+Qed.
+
+Lemma list_firstn_succ : forall A (l : list A) i d,
+  lt i (List.length l) ->
+  List.firstn (S i) l = (List.firstn i l ++l [List.nth i l d]).
+Proof.
+  induction l.
+  inversion 1.
+
+  lists.
+  intros.
+  destruct i.
+  lists.
+  replace ((S i + 1)%nat) with (S (i + 1)) by lia.
+  lists.
+  f_equal.
+  apply IHl.
+  lia.
+Qed.
+(* }}} *)
+
+
+
+
+Module bv.
+  Local Open Scope N_scope.
+  Definition zeroes (n : nat) : list N := List.repeat 0 n.
+
+  (* Pos *)
+  Local Open Scope positive_scope.
+  Compute 1~1~0.
+  Fixpoint of_pos (p : positive) : list N :=
+    match p with
+    | 1 => [1%N]
+    | p~0 => 0%N :: of_pos p
+    | p~1 => 1%N :: of_pos p
+    end.
+  Close Scope positive_scope.
+
+  (* N *)
+  Local Open Scope N_scope.
+  Definition of_N (n : N) : list N :=
+    match n with
+    | N0 => [0]
+    | Npos p => of_pos p
+    end.
+
+  Fixpoint to_N (bv : list N) : N :=
+    match bv with
+    | [] => 0
+    | h :: t => (to_N t) * 2 + h
+    end.
+
+  Lemma N_bv_equiv : forall n,
+    n = to_N (of_N n).
+  Proof.
+    destruct n; trivial; simpl.
+    induction p; simpl; try lia.
+  Qed.
+
+  (* zeroes *)
+  Lemma zeroes_is_zero : forall n,
+    to_N (zeroes n) = 0.
+  Proof.
+    unfold zeroes.
+    induction n; simpl; eauto.
+    rewrite IHn; lia.
+  Qed.
+
+  (* size *)
+  Lemma bv_size_equiv : forall n,
+    n <> 0
+    -> List.length (of_N n) = N.to_nat (N.size n).
+  Proof.
+    intros n HP.
+    induction n; simpl; try lia.
+    induction p; simpl; try lia.
+  Qed.
+
+  Lemma N_bv_nz : forall n,
+    (List.length (of_N n)) <> 0%nat.
+  Proof.
+    induction n; simpl; eauto.
+    induction p; simpl; eauto.
+  Qed.
+
+  Lemma Pos_size : forall n m,
+    Pos.le n m -> Pos.le (Pos.size n) (Pos.size m).
+  Proof.
+    induction n; simpl; try lia; intros;
+      induction m; simpl; try lia;
+        rewrite <- Pos.succ_le_mono; apply IHn; lia.
+  Qed.
+
+  Lemma N_size : forall n m,
+    n <= m -> N.size n <= N.size m.
+  Proof.
+    induction n; simpl; try lia.
+    induction m; simpl; try lia.
+    apply Pos_size.
+  Qed.
+
+  Lemma N_bv_add : forall n m,
+    n <> 0 /\ m <> 0
+    -> le (List.length (of_N (n + m)))
+    ((max (List.length (of_N n)) (List.length (of_N m))) + 1).
+  Proof.
+    intros.
+    rewrite! bv_size_equiv by lia.
+    destruct (N.leb n m) eqn:Heq.
+    - rewrite N.leb_le in Heq.
+      replace (Nat.max (N.to_nat (N.size n)) (N.to_nat (N.size m))) with (N.to_nat (N.max (N.size n) (N.size m))) by lia.
+
+      apply PeanoNat.Nat.le_trans with (m := (N.to_nat (N.size (2 * m + 1)))).
+      + rewrite! N.size_log2 by lia.
+        assert (N.log2 (n + m) <= N.log2 (2 * m + 1)).
+        apply N.log2_le_mono.
+        lia.
+        lia.
+      + rewrite! N.size_log2 by lia.
+        rewrite N.log2_succ_double by lia.
+        lia.
+
+    - Search (N.leb).
+      rewrite N.leb_gt in Heq.
+      replace (Nat.max (N.to_nat (N.size n)) (N.to_nat (N.size m))) with (N.to_nat (N.max (N.size n) (N.size m))) by lia.
+
+      apply PeanoNat.Nat.le_trans with (m := (N.to_nat (N.size (2 * n + 1)))).
+      + rewrite! N.size_log2 by lia.
+        assert (N.log2 (n + m) <= N.log2 (2 * n + 1)).
+        apply N.log2_le_mono.
+        lia.
+        lia.
+      + rewrite! N.size_log2 by lia.
+        rewrite N.log2_succ_double by lia.
+        lia.
+  Qed.
+
+  Lemma of_N_spec : forall n d i,
+    lt i (N.to_nat (N.size n))
+    -> List.nth i (bv.of_N n) d = N.b2n (N.testbit n (N.of_nat i)).
+  Proof.
+    induction n; simpl.
+    inversion 1.
+
+    induction p; simpl; destruct i; simpl; try lia;
+    intros;
+    assert ((i < Pos.to_nat (Pos.size p))%nat) by lia;
+    pose proof (IHp d _ H0);
+    rewrite H1;
+    f_equal;
+    f_equal;
+    lia.
+  Qed.
+
+  Close Scope N_scope.
+End bv.
+
+Module bvM.
+  (* Conversion {{{ *)
+  Definition of_N (m : nat) (n : N) : list N :=
+    if Nat.eqb m 0 then []
+    else 
+      let l := bv.of_N n in
+      let len := (List.length l) in
+      if Nat.leb len m then List.app l (bv.zeroes (m - len)) else List.firstn m l.
+
+  Lemma of_0 : forall b,
+    bvM.of_N b 0 = bv.zeroes b.
+  Proof.
+    induction b; simpl; eauto.
+    assert (S b <> O) by lia.
+    unfold of_N; simpl.
+    rewrite PeanoNat.Nat.sub_0_r.
+    unfold bv.zeroes; eauto.
+  Qed.
+
+  Lemma of_N_0 : forall n,
+    bvM.of_N 0 n = [].
+  Proof.
+    eauto.
+  Qed.
+
+  Lemma of_N_length : forall n m,
+    List.length (bvM.of_N m n) = m.
+  Proof.
+    induction m; simpl; eauto.
+    unfold bvM.of_N.
+    assert (Nat.eqb (S m) 0 = false).
+    rewrite PeanoNat.Nat.eqb_neq; lia.
+    Opaque List.firstn.
+    simpl.
+
+    destruct (Nat.leb (Datatypes.length (bv.of_N n)) (S m)) eqn:Hle.
+    - apply PeanoNat.Nat.leb_le in Hle.
+      rewrite List.app_length.
+      unfold bv.zeroes.
+      destruct (Datatypes.length (bv.of_N n)).
+      + rewrite List.repeat_length; eauto.
+      + rewrite List.repeat_length.
+        rewrite PeanoNat.Nat.add_sub_assoc; lia.
+    - destruct (Datatypes.length (bv.of_N n)) eqn:Heq.
+      + inversion Hle.
+      + apply PeanoNat.Nat.leb_gt in Hle.
+        rewrite <- Heq in Hle.
+        rewrite List.firstn_length.
+        apply min_l; lia.
+  Qed.
+
+  Lemma of_N_spec : forall i m n d,
+    lt i m
+    -> List.nth i (bvM.of_N m n) d = N.b2n (N.testbit n (N.of_nat i)).
+  Proof.
+    intros.
+    unfold bvM.of_N.
+    destruct (Nat.eqb m 0) eqn:Heq.
+    - rewrite PeanoNat.Nat.eqb_eq in Heq; lia.
+    - destruct (Nat.leb (Datatypes.length (bv.of_N n)) m) eqn:Hleb.
+      + rewrite PeanoNat.Nat.leb_le in Hleb.
+        destruct (N.eqb n 0) eqn:HN. 
+        * rewrite N.eqb_eq in HN.
+          subst; simpl.
+          destruct i eqn:Hi; eauto.
+          unfold bv.zeroes.
+          rewrite List.nth_indep with (d' := 0%N).
+          rewrite List.nth_repeat; eauto.
+          rewrite List.repeat_length; lia.
+        * rewrite N.eqb_neq in HN.
+          destruct (Nat.ltb i (List.length (bv.of_N n))) eqn:Hin.
+          { rewrite PeanoNat.Nat.ltb_lt in Hin.
+            rewrite List.app_nth1; eauto.
+            apply bv.of_N_spec.
+            rewrite <- bv.bv_size_equiv; lia. }
+          { rewrite PeanoNat.Nat.ltb_ge in Hin.
+            rewrite List.app_nth2; eauto.
+
+            unfold bv.zeroes.
+            rewrite List.nth_indep with (d' := 0%N).
+            rewrite List.nth_repeat; eauto.
+            rewrite bit_fact; simpl. lia.
+            rewrite bv.bv_size_equiv in Hin; lia.
+
+            rewrite List.repeat_length; lia. }
+      + rewrite PeanoNat.Nat.leb_gt in Hleb.
+        destruct (N.eqb n 0) eqn:HN. 
+        * rewrite N.eqb_eq in HN.
+          subst; simpl.
+          simpl in Hleb.
+          lia.
+        * rewrite N.eqb_neq in HN.
+          rewrite list_fact; try lia.
+          apply bv.of_N_spec.
+          rewrite bv.bv_size_equiv in Hleb; try lia.
+  Qed.
+
+  Lemma of_N_succ : forall m n,
+    bvM.of_N (S m) n = List.app (bvM.of_N m n) [N.b2n (N.testbit n (N.of_nat m))].
+  Proof.
+    intros.
+    eapply List.nth_ext.
+    - rewrite List.app_length.
+      rewrite! bvM.of_N_length.
+      simpl; lia.
+    - rewrite bvM.of_N_length.
+      intros.
+      destruct (Nat.ltb n0 m) eqn:ineq.
+      + rewrite PeanoNat.Nat.ltb_lt in ineq.
+        rewrite List.app_nth1; try reflexivity.
+        rewrite! bvM.of_N_spec; eauto.
+        rewrite bvM.of_N_length; lia.
+      + rewrite PeanoNat.Nat.ltb_ge in ineq.
+        assert (n0 = m) by lia; subst.
+        rewrite List.app_nth2; rewrite bvM.of_N_length; try lia.
+        rewrite! bvM.of_N_spec; eauto.
+        replace (m - m)%nat with O by lia; eauto.
+    Unshelve.
+    all: eauto.
+  Qed.
+  (* }}} *)
+
+  (* L-Shifting {{{ *)
+  (* }}} *)
+End bvM.
+
+Close Scope UROP_scope.
