ExtraArith.v
@@ -1,0 +1,42 @@
+Require Import NArith.
+Require Import UROP.Types.
+
+Require Import Lia.
+
+Local Open Scope N_scope.
+
+Lemma bit_fact : forall n i,
+  N.size n <= i -> N.testbit n i = false.
+Proof.
+  induction n; simpl; eauto.
+  induction p; simpl; destruct i; simpl; try lia;
+    intros;
+    assert (N.pos (Pos.size p) <= Pos.pred_N p0) by lia;
+    pose proof (IHp _ H0);
+    eauto.
+Qed.
+
+Lemma i_mod_plus_bit : forall i s,
+  i < 2 ^ (s + 1)
+  -> i mod 2 ^ s + N.b2n (N.testbit i s) * 2 ^ s = i.
+Proof.
+  intros.
+  rewrite N.testbit_eqb.
+  destruct (N.ltb i (2 ^ s)) eqn:Hlt.
+  - rewrite N.ltb_lt in Hlt.
+    rewrite N.mod_small; eauto.
+    replace (i / 2 ^ s) with 0; simpl; try rewrite N.div_small; lia.
+  - rewrite N.ltb_ge in Hlt.
+    rewrite N.mod_eq; try lia.
+    replace (i / 2 ^ s) with 1; simpl N.b2n; try lia.
+    assert (i / 2 ^ s < 2).
+    { apply N.div_lt_upper_bound; try lia.
+      rewrite N.mul_comm.
+      rewrite <- N.pow_succ_r; lia. }
+    assert (i / 2 ^ s > 0).
+    { apply N.lt_gt.
+      apply N.div_str_pos; lia. }
+    lia.
+Qed.
+
+Local Close Scope N_scope.
